various edits

code/loop-insecure.java
@@ -1,4 +1,4 @@
 int f(int h, int l) {
-  while (h>0) { h--; l++; }
+  while (h > 0) { h--; l++; }
   return l;
 }
