code/loop-secure.java
@@ -1,4 +1,4 @@
 int f(int h, int l) {
-  while (h>0) { h--; }
+  while (h > 0) { h--; }
   return l;
 }
