code/equiv.v
@@ -1,33 +1,197 @@
-Require Import Maps Imp.
-From Coq Require Import Arith.PeanoNat. Import Nat.
-From Coq Require Import Arith.EqNat.
+Set Warnings "-notation-overridden,-parsing,-deprecated-hint-without-locality".
+From Coq Require Import Arith.Arith.
+From Coq Require Import Arith.EqNat. Import Nat.
+From Coq Require Import Strings.String.
 
+(* ################################################################# *)
+(** * Total Maps and States *)
+
+Definition total_map (A : Type) := string -> A.
+
+Definition t_empty {A : Type} (v : A) : total_map A :=
+  (fun _ => v).
+
+Definition t_update {A : Type} (m : total_map A)
+                    (x : string) (v : A) :=
+  fun x' => if String.eqb x x' then v else m x'.
+
+Notation "'_' '!->' v" := (t_empty v)
+  (at level 100, right associativity).
+
+Notation "x '!->' v ';' m" := (t_update m x v)
+                              (at level 100, v at next level, right associativity).
+
+Definition state := total_map nat.
+
+Definition empty_st := (_ !-> 0).
+
+Notation "x '!->' v" := (x !-> v ; empty_st) (at level 100).
+
+(* ################################################################# *)
+(** * Imp: Simple Imperative Programs *)
+
+(** ** Syntax  *)
+Inductive aexp : Type :=
+  | ANum (n : nat)
+  | AId (x : string)              (* <--- NEW *)
+  | APlus (a1 a2 : aexp)
+  | AMinus (a1 a2 : aexp)
+  | AMult (a1 a2 : aexp).
+
+Inductive bexp : Type :=
+  | BTrue
+  | BFalse
+  | BEq (a1 a2 : aexp)
+  | BNeq (a1 a2 : aexp)
+  | BLe (a1 a2 : aexp)
+  | BGt (a1 a2 : aexp)
+  | BNot (b : bexp)
+  | BAnd (b1 b2 : bexp).
+
+Inductive com : Type :=
+  | CSkip
+  | CAsgn (x : string) (a : aexp)
+  | CSeq (c1 c2 : com)
+  | CIf (b : bexp) (c1 c2 : com)
+  | CWhile (b : bexp) (c : com).
+
+Definition X : string := "X".
+Definition Y : string := "Y".
+Definition Z : string := "Z".
+
+(** ** Notations *)
+
+Coercion AId : string >-> aexp.
+Coercion ANum : nat >-> aexp.
+
+Declare Custom Entry com.
+Declare Scope com_scope.
+Declare Custom Entry com_aux.
+
+Notation "<{ e }>" := e (e custom com_aux) : com_scope.
+Notation "e" := e (in custom com_aux at level 0, e custom com) : com_scope.
+
+Notation "( x )" := x (in custom com, x at level 99) : com_scope.
+Notation "x" := x (in custom com at level 0, x constr at level 0) : com_scope.
+Notation "f x .. y" := (.. (f x) .. y)
+                  (in custom com at level 0, only parsing,
+                  f constr at level 0, x constr at level 9,
+                  y constr at level 9) : com_scope.
+Notation "x + y"   := (APlus x y) (in custom com at level 50, left associativity).
+Notation "x - y"   := (AMinus x y) (in custom com at level 50, left associativity).
+Notation "x * y"   := (AMult x y) (in custom com at level 40, left associativity).
+Notation "'true'"  := true (at level 1).
+Notation "'true'"  := BTrue (in custom com at level 0).
+Notation "'false'" := false (at level 1).
+Notation "'false'" := BFalse (in custom com at level 0).
+Notation "x <= y"  := (BLe x y) (in custom com at level 70, no associativity).
+Notation "x > y"   := (BGt x y) (in custom com at level 70, no associativity).
+Notation "x = y"   := (BEq x y) (in custom com at level 70, no associativity).
+Notation "x <> y"  := (BNeq x y) (in custom com at level 70, no associativity).
+Notation "x && y"  := (BAnd x y) (in custom com at level 80, left associativity).
+Notation "'~' b"   := (BNot b) (in custom com at level 75, right associativity).
+
+Notation "'skip'"  :=
+         CSkip (in custom com at level 0) : com_scope.
+Notation "x := y"  :=
+         (CAsgn x y)
+            (in custom com at level 0, x constr at level 0,
+             y at level 85, no associativity) : com_scope.
+Notation "x ; y" :=
+         (CSeq x y)
+           (in custom com at level 90,
+            right associativity) : com_scope.
+Notation "'if' x 'then' y 'else' z 'end'" :=
+         (CIf x y z)
+           (in custom com at level 89, x at level 99,
+            y at level 99, z at level 99) : com_scope.
+Notation "'while' x 'do' y 'end'" :=
+         (CWhile x y)
+           (in custom com at level 89, x at level 99,
+            y at level 99) : com_scope.
 Open Scope com_scope.
 
-Definition aequiv (a1 a2 : aexp) : Prop :=
-  forall (st : state),  aeval st a1 = aeval st a2.
+(** ** Evaluation *)
+
+Fixpoint aeval (st : state) (a : aexp) : nat :=
+  match a with
+  | ANum n => n
+  | AId x => st x                                
+  | <{a1 + a2}> => (aeval st a1) + (aeval st a2)
+  | <{a1 - a2}> => (aeval st a1) - (aeval st a2)
+  | <{a1 * a2}> => (aeval st a1) * (aeval st a2)
+  end.
+
+Fixpoint beval (st : state) 
+               (b : bexp) : bool :=
+  match b with
+  | <{true}>      => true
+  | <{false}>     => false
+  | <{a1 = a2}>   => (aeval st a1) =? (aeval st a2)
+  | <{a1 <> a2}>  => negb ((aeval st a1) =? (aeval st a2))
+  | <{a1 <= a2}>  => (aeval st a1) <=? (aeval st a2)
+  | <{a1 > a2}>   => negb ((aeval st a1) <=? (aeval st a2))
+  | <{~ b1}>      => negb (beval st b1)
+  | <{b1 && b2}>  => andb (beval st b1) (beval st b2)
+  end.
+
+Reserved Notation
+         "st '=[' c ']=>' st'"
+         (at level 40, c custom com at level 99,
+          st constr, st' constr at next level).
+
+Inductive ceval : com -> state -> state -> Prop :=
+  | E_Skip : forall st,
+      st =[ skip ]=> st
+  | E_Asgn  : forall st a n x,
+      aeval st a = n ->
+      st =[ x := a ]=> (x !-> n ; st)
+  | E_Seq : forall c1 c2 st st' st'',
+      st  =[ c1 ]=> st'  ->
+      st' =[ c2 ]=> st'' ->
+      st  =[ c1 ; c2 ]=> st''
+  | E_IfTrue : forall st st' b c1 c2,
+      beval st b = true ->
+      st =[ c1 ]=> st' ->
+      st =[ if b then c1 else c2 end]=> st'
+  | E_IfFalse : forall st st' b c1 c2,
+      beval st b = false ->
+      st =[ c2 ]=> st' ->
+      st =[ if b then c1 else c2 end]=> st'
+  | E_WhileFalse : forall b st c,
+      beval st b = false ->
+      st =[ while b do c end ]=> st
+  | E_WhileTrue : forall st st' st'' b c,
+      beval st b = true ->
+      st  =[ c ]=> st' ->
+      st' =[ while b do c end ]=> st'' ->
+      st  =[ while b do c end ]=> st''
+
+  where "st =[ c ]=> st'" := (ceval c st st').
+
+(* ################################################################# *)
+(** ** Equivalence *)
 
 Definition equiv (c1 c2 : com) : Prop :=
-  forall (st st' : state), (st =[ c1 ]=> st') <-> (st =[ c2 ]=> st').
+  forall (st st' : state),
+  (st =[ c1 ]=> st') <-> (st =[ c2 ]=> st').
 
-Notation "p '===' q" :=
-  (cequiv p q) (at level 50, left associativity).
-
-Theorem prog_eq b X Y Z :
+Theorem program_equivalence (b: nat) (X Y : aexp) (Z : string) :
     b = 0 \/ b = 1 ->
-    <{ if b = 1 then Z := X else Z := Y end }>
-    === <{ Z := X * b + Y * (1 - b) }>.
+    equiv <{ if b = 1 then Z := X else Z := Y end }>
+          <{ Z := X * b + Y * (1 - b) }>.
 Proof.
   intros; split.
-  (* if ... *)
+  (* if ... -> Z := ... *)
   - intros C1; inversion C1; subst; clear C1;
       inversion H; subst; try discriminate;
-      inversion H6; subst; apply E_Asgn; simpl;
-      rewrite mul_0_r, mul_1_r; auto.
-  (* Z := ... *)
-  - intros C2; destruct H as [H|H]; subst;
-      [apply E_IfFalse|apply E_IfTrue]; auto;
-      inversion C2; subst; clear C2;
+      inversion H6; subst;
       apply E_Asgn; simpl;
       rewrite mul_0_r, mul_1_r; auto.
-Qed.    
+  (* Z := ... ->  if ... *)
+  - intros C2; destruct H as [H|H]; subst;
+      [apply E_IfFalse|apply E_IfTrue]; auto;
+      inversion C2; subst; 
+      apply E_Asgn; simpl;
+      rewrite mul_0_r, mul_1_r; auto.
+Qed.
