code/leftpad-ssrefl.v
@@ -1,28 +1,25 @@
-Set Warnings "-notation-overridden".
 From mathcomp Require Import ssreflect ssrbool ssrnat seq.
-Set Implicit Arguments.
-Unset Strict Implicit.
-Unset Printing Implicit Defensive.
 
 Section LeftPad.
+  Variables (T : Type) (def : T).  
+  Implicit Types (c : T) (n : nat) (s : seq T).
+  Local Notation nth := (nth def).  (* nth list element *)
 
-(* [def] is the default value, i.e. type T is not empty *)
-Variables (T : Type) (def : T).
-Local Notation nth := (nth def)  (* n-th element of list *)
+  Definition leftpad c n s : seq T :=
+      ncons (n - size s) c s.
 
-Definition leftpad (c : T) (n : nat) (s : seq T) : seq T :=
-  ncons (n - size s) c s.
+  Lemma length_max_spec c n s :
+    size (leftpad c n s) = maxn n (size s).
+  Proof. by rewrite size_ncons addnC maxnC maxnE. Qed.
 
-Lemma length_max_spec c n s :
-  size (leftpad c n s) = maxn n (size s).
-Proof. by rewrite size_ncons addnC maxnC maxnE. Qed.
+  Lemma prefix_spec c n s : forall i,
+    i < n - size s -> nth (leftpad c n s) i = c.
+  Proof. by move=> i; rewrite nth_ncons => -> . Qed.
 
-Lemma prefix_spec c n s :
-  forall i, i < n - size s -> nth (leftpad c n s) i = c.
-Proof. by move=> i; rewrite nth_ncons => ->. Qed.
-
-Lemma suffix_spec c n s : forall i,
-  i < size s -> nth (leftpad c n s) (n - size s + i) = nth s i.
-Proof. by move=> i _; rewrite nth_ncons addKn ifN // -ltnNge leq_addr. Qed.
-
+  Lemma suffix_spec c n s : forall i,
+      i < size s ->
+      nth (leftpad c n s) (n - size s + i) = nth s i.
+  Proof.
+    by move=> i _; rewrite nth_ncons addKn ifN//-ltnNge leq_addr.
+  Qed.
 End LeftPad.
