code/leftpad.dfy
@@ -1,13 +1,12 @@
-function Max(a: int, b: int): int
-{
+function Max(a: int, b: int): int {
   if a > b then a else b
 }
 
 method LeftPad(c: char, n: int, s: seq<char>)
   returns (v: seq<char>)
-  ensures |v| == Max(n, |s|)
-  ensures forall i :: 0 <= i < n - |s| ==> v[i] == c
-  ensures forall i :: 0 <= i < |s| ==> v[Max(n - |s|, 0) + i] == s[i]
+  ensures |v| == Max(n, |s|) 
+  ensures forall i :: 0 <= i < n - |s| ==> v[i] == c  
+  ensures forall i :: 0 <= i < |s| ==> v[Max(n - |s|, 0) + i] == s[i] 
 {
   var pad, i := Max(n - |s|, 0), 0;
   v := s;
@@ -21,11 +20,4 @@ method LeftPad(c: char, n: int, s: seq<char>)
     v := [c] + v;
     i := i + 1;
   }
-}
-
-method Main() {
-  var l1 := LeftPad('0', 5, "foo");
-  var l2 := LeftPad('0', 1, "foo");
-  print l1 + "\n\n";
-  print l2;
 }
