code/leftpad.cmd
@@ -1,0 +1,3 @@
+leftpad('!', 5, "wow")
+leftpad('!', 0, "wow")
+leftpad('?', 4, "wow")
